Specify well-formed terms

theories/Terms.v
@@ -3,6 +3,7 @@ From QuickChick Require Import QuickChick.
 From Coq Require Import String.
 From LambdaST Require Import
   Eqb
+  Sets
   Types.
 
 Declare Scope term_scope.
@@ -51,3 +52,53 @@ Instance eqb_term : Eqb term := { eqb := term_beq; eq_dec := term_eq_dec; eqb_sp
 Hint Unfold term_beq : core.
 Hint Resolve term_eq_dec : core.
 Hint Resolve eqb_spec_term : core.
+
+Inductive WFTerm : set string -> term -> Prop :=
+  | WFTmSink : forall s,
+      WFTerm s TmSink
+  | WFTmUnit : forall s,
+      WFTerm s TmUnit
+  | WFTmVar : forall x s,
+      s x ->
+      WFTerm s (TmVar x)
+  | WFTmComma : forall e e' s,
+      WFTerm s e ->
+      WFTerm s e' ->
+      WFTerm s (e, e')
+  | WFTmSemic : forall e e' s,
+      WFTerm s e ->
+      WFTerm s e' ->
+      WFTerm s (e; e')
+  | WFTmLet : forall x e e' s,
+      ~s x ->
+      (* is this right? *)
+      WFTerm s e ->
+      WFTerm (set_union s (singleton_set x)) e' ->
+      WFTerm s (TmLet x e e')
+  | WFTmLetPar : forall x y z e s,
+      WFTerm (set_union (set_minus s (singleton_set z)) (set_union (singleton_set x) (singleton_set y))) e ->
+      s z ->
+      ~s x ->
+      ~s y ->
+      x <> y ->
+      WFTerm s (TmLetPar x y z e)
+  | WFTmLetCat : forall x y z e t s,
+      WFTerm (set_union (set_minus s (singleton_set z)) (set_union (singleton_set x) (singleton_set y))) e ->
+      s z ->
+      ~s x ->
+      ~s y ->
+      x <> y ->
+      (* TODO: WFType s t -> *)
+      WFTerm s (TmLetCat t x y z e)
+.
+Hint Constructors WFTerm : core.
+
+Theorem wf_iff : forall s s' e,
+  SetEq s s' ->
+  WFTerm s e ->
+  WFTerm s' e.
+Proof.
+  intros.
+  generalize dependent s'.
+  induction H0; cbn in *; intros; constructor; sfirstorder.
+Qed.
